rustdemo/LinkedListSafe.v
@@ -77,9 +77,15 @@ Inductive return_find : state -> Prop :=
 
 Fixpoint num_frames_cont (k: cont) : nat :=
   match k with
+  | Kstop => O
   | Kcall _ _ _ _ k' =>
       S (num_frames_cont k')
-  | _ => O
+  | Kseq _ k
+  | Kloop _ k
+  | Kdropinsert _ _ k
+  | Kdropplace _ _ _ _ _ k
+  | Kdropcall _ _ _ _ k
+  | Klet _ _ k => num_frames_cont k
   end.
 
 Definition num_frames (s: state) : nat :=
@@ -97,14 +103,14 @@ Inductive sound_state : state -> Prop :=
 | find_state_internal1: forall s0 s1 t n
     (CALL: call_func find s0)
     (STAR: starN step ge n s0 t s1)
-    (RAN: (0 <= n <= 3)%nat)
+    (RAN: (0 <= n <= 20)%nat)
     (* all execution is inside the current function *)
     (NUMF: num_frames s0 = num_frames s1),
     sound_state s1
 | find_state_internal2: forall s0 s1 t n,
     return_find s0 ->
     starN step ge n s0 t s1 ->
-    (0 <= n <= 3)%nat ->  
+    (0 <= n <= 10)%nat ->  
     num_frames s0 = num_frames s1 ->
     sound_state s1
 | find_returnstate: forall v k m,
@@ -147,7 +153,7 @@ Lemma init_own_env_find_progress:
               (map
                  (fun elt : ident * type => Plocal (fst elt) (snd elt))
                  (fn_params find_func ++ fn_vars find_func))))) in *.
-  change (check_own_env_consistency
+  replace (check_own_env_consistency
         (PTree.map
            (fun (_ : positive) (_ : InitDomain.LPaths.t) =>
             InitDomain.Paths.empty)
@@ -208,11 +214,33 @@ Lemma init_own_env_find_progress:
               (map
                  (fun elt : ident * type => Plocal (fst elt) (snd elt))
                  (fn_params find_func ++ fn_vars find_func))))) with true in *. congruence.
-  (* reflexivity. *)
+  reflexivity.
   congruence.
   unfold collect_func in A. congruence.
 Qed.
-                                                                                
+
+        
+Lemma function_entry_find_progress: forall vl m1,
+    length_of_args find = length vl ->
+  exists e m2, function_entry ge find_func vl m1 e m2.
+Admitted.
+
+(* Compute (variant_field_offset (proj1_sig build_ce_ok) Nil [Member_plain Nil Tunit; Member_plain Cons Node_ty]). *)
+
+
+Definition val_is_ptr (v: val) : bool :=
+  match v with
+  | Vptr _ _ => true
+  | _ => false
+  end.
+
+
+Definition val_is_int (v: val) : bool :=
+  match v with
+  | Vint _ => true
+  | _ => false
+  end.
+
 Lemma step_preservation_progress: forall s,
     sound_state s ->
     (not_stuck (linked_list_sem se) s \/ step_mem_error ge s)
@@ -233,10 +261,144 @@ Proof.
     (* take zero step *)
     { split.
       - left. red. right. right.
+        edestruct (function_entry_find_progress vl m) as (e & m1 & ENT); eauto.
+        destruct init_own_env_find_progress as (own & INITOWN).
         do 2 eexists.
         econstructor; eauto.
+      - intros. eapply find_state_internal1 with (n:= 1%nat); eauto.
+        econstructor; eauto. econstructor. lia.
+        inv H; simpl; auto. }
+    (** take one step *)
+    inv H; try congruence.
+    rewrite FIND in FIND0. inv FIND0.    
+    unfold init_own_env in INITOWN.
+    (* construct own_env *)
+    destruct collect_func eqn: A; cbn [bind] in INITOWN; try congruence.
+    set (empty_map := (PTree.map
+                         (fun (_ : positive) (_ : InitDomain.LPaths.t) =>
+                            InitDomain.Paths.empty) t)) in *.
+    set (initParams:= (InitDomain.add_place_list t
+                         (places_of_locals (fn_params find_func ++ fn_vars find_func))
+                       empty_map)) in *.
+    set (flag := check_own_env_consistency empty_map empty_map initParams t) in *.
+    generalize INITOWN. clear INITOWN.
+    generalize (eq_refl flag).
+    generalize flag at 1 3.
+    intros flag0 E. destruct flag0; try congruence. intros. inv INITOWN.
+    (* construct e *)
+    inv ENTRY. inv ALLOC. inv H8. inv H10. inv H11. inv H12. inv H13.
+    inv H14. inv H15. inv H16. inv H17.
+    inv H0.
+    (* stop here: evaluate the if statement *)
+    { split.
+      - left. red.
+        (** decide whether there would be memory error  *)
+        destruct (Mem.valid_access_dec m' Mptr b1 0 Readable) eqn: VA1.
+        + exploit Mem.valid_access_load. eapply v. intros (v1 & LOAD1).
+          (* we should show thata v1 must be a pointer *)
+          destruct (val_is_ptr v1) eqn: VPTR.
+          * destruct v1; simpl in VPTR; try congruence.
+            destruct (Mem.valid_access_dec m' Mint32 b9 (Ptrofs.unsigned i) Readable) eqn: VA2.
+            -- exploit Mem.valid_access_load. eapply v0. intros (v2 & LOAD2).
+               destruct (val_is_int v2) eqn: VINT.
+               ++ destruct v2; simpl in VINT; try congruence.
+                  right. right.
+                  
+                  do 2 eexists.
+                  (* evaluate if then else *)
+                  econstructor. econstructor. econstructor. econstructor.
+                  econstructor.
+                  do 8 (try rewrite PTree.gso; try (cbv delta; congruence)).
+                  rewrite PTree.gss. reflexivity.
+                  econstructor. simpl. eauto.
+                  eauto. eauto. simpl. unfold List_ty. eauto.
+                  simpl. reflexivity. reflexivity.
+                  reflexivity.
+                  simpl.
+                  instantiate (1 := Int.eq i0 (Int.repr 0)).
+                  destruct (Int.eq i0 (Int.repr 0)) eqn: EQZ; reflexivity.
+               (* The tag is not an Int value *)
+               ++ admit.
+            (* The memory location of tag is not loadable *)
+            -- admit.
+          (* The value loaded from the place is not a pointer *)
+          * admit.
+        (* The block of l is not loadable *)
+        + admit.
+      (* Invariant preservation *)
+      - intros. eapply find_state_internal1 with (n:=2%nat); eauto.
+        eapply starN_step_right; eauto. lia.
+        inv H; simpl; auto. }
+    (* destruct the if step *)
+    inv H.
+    2: { destruct H18; unfold find_body in *; try congruence. }
+    (* get the bool value *)
+    simpl in H22. inv H20. inv H0.
+    simpl in H5. unfold List_ty in H5. inv H5. simpl in H6.
+    rewrite PTree.gss in H6. inv H6. simpl in H17.
+    vm_compute in H17. inv H17.
+    destruct (Int.eq tag (Int.repr 0)) eqn: EQZ; vm_compute in H22; inv H22.
+    (** evaluate the if branch *)
+    { inv H1.
+      (* stop here: evaluate Slet *)
+      { split.
+        - left. red. do 2 right.
+          do 2 eexists. econstructor.
+        - intros. eapply find_state_internal1 with (n:=3%nat); eauto.
+          eapply starN_step_right; eauto. lia.
+          inv H; simpl; auto. }
+      inv H.
+      2: { destruct H20; try congruence. }
+      inv H0.
+      (* stop here: evaluate ssequence *)
+      { split.
+        - left. red. do 2 right.
+          do 2 eexists. econstructor.
+        - intros. eapply find_state_internal1 with (n:=4%nat); eauto.
+          eapply starN_step_right; eauto. lia.
+          inv H; simpl; auto. }
+      inv H. inv H1.
+      (* stop here: evaluate to Dassign *)
+      { split.
+        - left. red. do 2 right.
+          do 2 eexists. econstructor.
+        - intros. eapply find_state_internal1 with (n:=5%nat); eauto.
+          eapply starN_step_right; eauto. lia.
+          inv H; simpl; auto. }
+      inv H. inv H0.
+      (* stop here: evaluate step_dropinsert_skip_reassign *)
+      { split.
+        - left. red. do 2 right.
+          do 2 eexists. econstructor.
+          eapply step_dropinsert_skip_reassign; auto.
+        - intros. eapply find_state_internal1 with (n:=6%nat); eauto.
+          eapply starN_step_right; eauto. lia.
+          inv H; inv SDROP; simpl; auto. }
+      inv H. inv SDROP; vm_compute in OWNTY; try congruence.
+      inv H1.
+      (* stop here: ealuate step_dropinsert_assign *)
+      { split.
+        - left. red. do 2 right.
+          do 2 eexists. econstructor.
+          eapply step_dropinsert_assign; auto.
+          simpl. congruence.
+          econstructor. reflexivity.
+          (* evaluate *l *)
+          econstructor. econstructor. econstructor.
+          eauto. reflexivity. reflexivity. eauto.
+          replace tag with (Int.repr 0). reflexivity.
+          generalize (Int.eq_spec tag (Int.repr 0)). rewrite EQZ. auto.
+          simpl. instantiate (1 := 8). reflexivity.
+          econstructor. simpl. eauto.
+          Mem.load_cast
+          Int.eq_
+          reflexivity.
+          repeat econstructor. 
+        Lemma starN_step_r: forall genv step 
         
-
+        econstructor.
+        Mem.valid_access_load
+    
         Lemma init_own_env_find_progress:
           exists own, init_own_env (Smallstep.globalenv (linked_list_sem se)) find_func =
  OK own.
