common/Smallstep.v
@@ -297,6 +297,11 @@ Proof.
   destruct IHstar as [n P]. exists (S n); econstructor; eauto.
 Qed.
 
+Remark starN_step_right ge: forall n s t t1 s' t2 s'',
+    starN ge n s t1 s' -> step ge s' t2 s'' -> t = t1 ** t2 ->
+    starN ge (S n) s t s''.
+Admitted.
+
 (** Infinitely many transitions *)
 
 CoInductive forever (ge: genv): state -> traceinf -> Prop :=
